Newly generated Boogie code.

tests/AddDelay.bpl
@@ -11,15 +11,15 @@ type Obj = <a>[Field a]a;
 type HType = [Ref]Obj;
 type ModeType = [Actor]int;
 
-var M: MType;
-var C: CType;
-var R: CType;
-var I: CType;
-var B: CType;
-var Mode: ModeType;
+var M#: MType;
+var C#: CType;
+var R#: CType;
+var I#: CType;
+var B#: CType;
+var Mode#: ModeType;
 var I#sub: CType;
 
-var H: HType;
+var H#: HType;
 
 const unique this#: Actor;
 
@@ -30,18 +30,18 @@ function AT#Min(x:int, y: int): int { if x <= y then x else y }
 // ---------------------------------------------------------------
 
 procedure Add#init#0()
-  modifies C, R, M, I, H, I#sub;
+  modifies C#, R#, M#, I#, H#, I#sub;
 {
   var in1: Chan (int);
   var in2: Chan (int);
   var out: Chan (int);
   assume (in1 != in2) && (in1 != out) && (in2 != out);
-  assume (I[in1] == 0) && (R[in1] == 0) && (C[in1] == 0);
-  assume (I[in2] == 0) && (R[in2] == 0) && (C[in2] == 0);
-  assume (I[out] == 0) && (R[out] == 0) && (C[out] == 0);
+  assume (I#[in1] == 0) && (R#[in1] == 0) && (C#[in1] == 0);
+  assume (I#[in2] == 0) && (R#[in2] == 0) && (C#[in2] == 0);
+  assume (I#[out] == 0) && (R#[out] == 0) && (C#[out] == 0);
 }
 procedure Add#anon$0#1()
-  modifies C, R, M, I, H, I#sub;
+  modifies C#, R#, M#, I#, H#, I#sub;
 {
   var in1: Chan (int);
   var in2: Chan (int);
@@ -49,97 +49,97 @@ procedure Add#anon$0#1()
   var in1#0: int;
   var in2#0: int;
   assume (in1 != in2) && (in1 != out) && (in2 != out);
-  assume (0 <= I[in1]) && (I[in1] <= R[in1]) && (R[in1] <= C[in1]);
-  assume (0 <= I[in2]) && (I[in2] <= R[in2]) && (R[in2] <= C[in2]);
-  assume (0 <= I[out]) && (I[out] <= R[out]) && (R[out] <= C[out]);
-  assume R[in1] == C[out];
-  assume R[in2] == C[out];
+  assume (0 <= I#[in1]) && (I#[in1] <= R#[in1]) && (R#[in1] <= C#[in1]);
+  assume (0 <= I#[in2]) && (I#[in2] <= R#[in2]) && (R#[in2] <= C#[in2]);
+  assume (0 <= I#[out]) && (I#[out] <= R#[out]) && (R#[out] <= C#[out]);
+  assume R#[in1] == C#[out];
+  assume R#[in2] == C#[out];
   assume (forall idx$: int :: 
-    (0 <= idx$) && (idx$ < C[out]) ==> (M[out][idx$] == (M[in1][idx$] + M[in2][idx$]))
+    (0 <= idx$) && (idx$ < C#[out]) ==> (M#[out][idx$] == (M#[in1][idx$] + M#[in2][idx$]))
   );
-  assume (1 <= (C[in1] - R[in1])) && (1 <= (C[in2] - R[in2]));
-  in1#0 := M[in1][R[in1]];
-  R[in1] := R[in1] + 1;
-  in2#0 := M[in2][R[in2]];
-  R[in2] := R[in2] + 1;
+  assume (1 <= (C#[in1] - R#[in1])) && (1 <= (C#[in2] - R#[in2]));
+  in1#0 := M#[in1][R#[in1]];
+  R#[in1] := R#[in1] + 1;
+  in2#0 := M#[in2][R#[in2]];
+  R#[in2] := R#[in2] + 1;
   assume true;
-  M[out][C[out]] := in1#0 + in2#0;
-  C[out] := C[out] + 1;
+  M#[out][C#[out]] := in1#0 + in2#0;
+  C#[out] := C#[out] + 1;
 }
 procedure Split#init#2()
-  modifies C, R, M, I, H, I#sub;
+  modifies C#, R#, M#, I#, H#, I#sub;
 {
   var in: Chan (int);
   var out1: Chan (int);
   var out2: Chan (int);
   assume (in != out1) && (in != out2) && (out1 != out2);
-  assume (I[in] == 0) && (R[in] == 0) && (C[in] == 0);
-  assume (I[out1] == 0) && (R[out1] == 0) && (C[out1] == 0);
-  assume (I[out2] == 0) && (R[out2] == 0) && (C[out2] == 0);
+  assume (I#[in] == 0) && (R#[in] == 0) && (C#[in] == 0);
+  assume (I#[out1] == 0) && (R#[out1] == 0) && (C#[out1] == 0);
+  assume (I#[out2] == 0) && (R#[out2] == 0) && (C#[out2] == 0);
 }
 procedure Split#anon$1#3()
-  modifies C, R, M, I, H, I#sub;
+  modifies C#, R#, M#, I#, H#, I#sub;
 {
   var in: Chan (int);
   var out1: Chan (int);
   var out2: Chan (int);
   var in#0: int;
   assume (in != out1) && (in != out2) && (out1 != out2);
-  assume (0 <= I[in]) && (I[in] <= R[in]) && (R[in] <= C[in]);
-  assume (0 <= I[out1]) && (I[out1] <= R[out1]) && (R[out1] <= C[out1]);
-  assume (0 <= I[out2]) && (I[out2] <= R[out2]) && (R[out2] <= C[out2]);
-  assume R[in] == C[out1];
-  assume R[in] == C[out2];
+  assume (0 <= I#[in]) && (I#[in] <= R#[in]) && (R#[in] <= C#[in]);
+  assume (0 <= I#[out1]) && (I#[out1] <= R#[out1]) && (R#[out1] <= C#[out1]);
+  assume (0 <= I#[out2]) && (I#[out2] <= R#[out2]) && (R#[out2] <= C#[out2]);
+  assume R#[in] == C#[out1];
+  assume R#[in] == C#[out2];
   assume (forall idx$: int :: 
-    (0 <= idx$) && (idx$ < C[out1]) ==> (M[out1][idx$] == M[in][idx$])
+    (0 <= idx$) && (idx$ < C#[out1]) ==> (M#[out1][idx$] == M#[in][idx$])
   );
   assume (forall idx$: int :: 
-    (0 <= idx$) && (idx$ < C[out2]) ==> (M[out2][idx$] == M[in][idx$])
+    (0 <= idx$) && (idx$ < C#[out2]) ==> (M#[out2][idx$] == M#[in][idx$])
   );
-  assume 1 <= (C[in] - R[in]);
-  in#0 := M[in][R[in]];
-  R[in] := R[in] + 1;
+  assume 1 <= (C#[in] - R#[in]);
+  in#0 := M#[in][R#[in]];
+  R#[in] := R#[in] + 1;
   assume true;
-  M[out1][C[out1]] := in#0;
-  C[out1] := C[out1] + 1;
-  M[out2][C[out2]] := in#0;
-  C[out2] := C[out2] + 1;
+  M#[out1][C#[out1]] := in#0;
+  C#[out1] := C#[out1] + 1;
+  M#[out2][C#[out2]] := in#0;
+  C#[out2] := C#[out2] + 1;
 }
 procedure Delay#init#4()
-  modifies C, R, M, I, H, I#sub;
+  modifies C#, R#, M#, I#, H#, I#sub;
 {
   var in: Chan (int);
   var out: Chan (int);
   var k: int;
   assume in != out;
-  assume (I[in] == 0) && (R[in] == 0) && (C[in] == 0);
-  assume (I[out] == 0) && (R[out] == 0) && (C[out] == 0);
-  M[out][C[out]] := k;
-  C[out] := C[out] + 1;
+  assume (I#[in] == 0) && (R#[in] == 0) && (C#[in] == 0);
+  assume (I#[out] == 0) && (R#[out] == 0) && (C#[out] == 0);
+  M#[out][C#[out]] := k;
+  C#[out] := C#[out] + 1;
 }
 procedure Delay#anon$3#5()
-  modifies C, R, M, I, H, I#sub;
+  modifies C#, R#, M#, I#, H#, I#sub;
 {
   var in: Chan (int);
   var out: Chan (int);
   var k: int;
   var in#0: int;
   assume in != out;
-  assume (0 <= I[in]) && (I[in] <= R[in]) && (R[in] <= C[in]);
-  assume (0 <= I[out]) && (I[out] <= R[out]) && (R[out] <= C[out]);
-  assume R[in] == (C[out] - 1);
+  assume (0 <= I#[in]) && (I#[in] <= R#[in]) && (R#[in] <= C#[in]);
+  assume (0 <= I#[out]) && (I#[out] <= R#[out]) && (R#[out] <= C#[out]);
+  assume R#[in] == (C#[out] - 1);
   assume (forall idx$: int :: 
-    (1 <= idx$) && (idx$ < C[out]) ==> (M[out][idx$] == M[in][idx$ - 1])
+    (1 <= idx$) && (idx$ < C#[out]) ==> (M#[out][idx$] == M#[in][idx$ - 1])
   );
-  assume 1 <= (C[in] - R[in]);
-  in#0 := M[in][R[in]];
-  R[in] := R[in] + 1;
+  assume 1 <= (C#[in] - R#[in]);
+  in#0 := M#[in][R#[in]];
+  R#[in] := R#[in] + 1;
   assume true;
-  M[out][C[out]] := in#0;
-  C[out] := C[out] + 1;
+  M#[out][C#[out]] := in#0;
+  C#[out] := C#[out] + 1;
 }
 procedure Net#init#6()
-  modifies C, R, M, I, H, I#sub;
+  modifies C#, R#, M#, I#, H#, I#sub;
 {
   var Net#add: Actor;
   var Net#del: Actor;
@@ -151,47 +151,47 @@ procedure Net#init#6()
   var Net#e: Chan (int);
   assume (Net#add != Net#del) && (Net#add != Net#spl) && (Net#del != Net#spl);
   assume (Net#a != Net#b) && (Net#a != Net#c) && (Net#a != Net#d) && (Net#a != Net#e) && (Net#b != Net#c) && (Net#b != Net#d) && (Net#b != Net#e) && (Net#c != Net#d) && (Net#c != Net#e) && (Net#d != Net#e);
-  assume 0 <= I[Net#a];
-  assume I[Net#a] <= R[Net#a];
-  assume R[Net#a] <= C[Net#a];
-  assume 0 <= I[Net#b];
-  assume I[Net#b] <= R[Net#b];
-  assume R[Net#b] <= C[Net#b];
-  assume 0 <= I[Net#c];
-  assume I[Net#c] <= R[Net#c];
-  assume R[Net#c] <= C[Net#c];
-  assume 0 <= I[Net#d];
-  assume I[Net#d] <= R[Net#d];
-  assume R[Net#d] <= C[Net#d];
-  assume I[Net#d] == R[Net#d];
-  assume 0 <= I[Net#e];
-  assume I[Net#e] <= R[Net#e];
-  assume R[Net#e] <= C[Net#e];
-  assume (B[Net#a] == 1) && (B[Net#d] == 1);
-  assume C[Net#a] == 0;
-  assume R[Net#a] == 0;
-  assume C[Net#b] == 0;
-  assume R[Net#b] == 0;
-  assume C[Net#c] == 0;
-  assume R[Net#c] == 0;
-  assume C[Net#d] == 0;
-  assume R[Net#d] == 0;
-  assume C[Net#e] == 0;
-  assume R[Net#e] == 0;
+  assume 0 <= I#[Net#a];
+  assume I#[Net#a] <= R#[Net#a];
+  assume R#[Net#a] <= C#[Net#a];
+  assume 0 <= I#[Net#b];
+  assume I#[Net#b] <= R#[Net#b];
+  assume R#[Net#b] <= C#[Net#b];
+  assume 0 <= I#[Net#c];
+  assume I#[Net#c] <= R#[Net#c];
+  assume R#[Net#c] <= C#[Net#c];
+  assume 0 <= I#[Net#d];
+  assume I#[Net#d] <= R#[Net#d];
+  assume R#[Net#d] <= C#[Net#d];
+  assume I#[Net#d] == R#[Net#d];
+  assume 0 <= I#[Net#e];
+  assume I#[Net#e] <= R#[Net#e];
+  assume R#[Net#e] <= C#[Net#e];
+  assume (B#[Net#a] == 1) && (B#[Net#d] == 1);
+  assume C#[Net#a] == 0;
+  assume R#[Net#a] == 0;
+  assume C#[Net#b] == 0;
+  assume R#[Net#b] == 0;
+  assume C#[Net#c] == 0;
+  assume R#[Net#c] == 0;
+  assume C#[Net#d] == 0;
+  assume R#[Net#d] == 0;
+  assume C#[Net#e] == 0;
+  assume R#[Net#e] == 0;
   assume 0 == 0;
-  M[Net#b][C[Net#b]] := 0;
-  C[Net#b] := C[Net#b] + 1;
-  assert {:msg "AddDelay.actor(24.15): Initialization of network 'Net' might not establish the channel invariant (#0)"} M[Net#b][0] == 0;
-  assert {:msg "AddDelay.actor(25.15): Initialization of network 'Net' might not establish the channel invariant (#1)"} 0 <= M[Net#b][I[Net#b]];
-  I := R;
-  assert {:msg "AddDelay.actor(23.13): Initialization of network 'Net' might not establish the network invariant (#2)"} (C[Net#b] - R[Net#b]) == 1;
-  assert {:msg "Initialization of network 'Net' might not establish the network invariant: Unread tokens might be left on channel a (#3)"} (C[Net#a] - R[Net#a]) == 0;
-  assert {:msg "Initialization of network 'Net' might not establish the network invariant: Unread tokens might be left on channel c (#4)"} (C[Net#c] - R[Net#c]) == 0;
-  assert {:msg "Initialization of network 'Net' might not establish the network invariant: Unread tokens might be left on channel d (#5)"} (C[Net#d] - R[Net#d]) == 0;
-  assert {:msg "Initialization of network 'Net' might not establish the network invariant: Unread tokens might be left on channel e (#6)"} (C[Net#e] - R[Net#e]) == 0;
+  M#[Net#b][C#[Net#b]] := 0;
+  C#[Net#b] := C#[Net#b] + 1;
+  assert {:msg "AddDelay.actor(24.15): Initialization of network 'Net' might not establish the channel invariant (#0)"} M#[Net#b][0] == 0;
+  assert {:msg "AddDelay.actor(25.15): Initialization of network 'Net' might not establish the channel invariant (#1)"} 0 <= M#[Net#b][I#[Net#b]];
+  I# := R#;
+  assert {:msg "AddDelay.actor(23.13): Initialization of network 'Net' might not establish the network invariant (#2)"} (C#[Net#b] - R#[Net#b]) == 1;
+  assert {:msg "Initialization of network 'Net' might not establish the network invariant: Unread tokens might be left on channel a (#3)"} (C#[Net#a] - R#[Net#a]) == 0;
+  assert {:msg "Initialization of network 'Net' might not establish the network invariant: Unread tokens might be left on channel c (#4)"} (C#[Net#c] - R#[Net#c]) == 0;
+  assert {:msg "Initialization of network 'Net' might not establish the network invariant: Unread tokens might be left on channel d (#5)"} (C#[Net#d] - R#[Net#d]) == 0;
+  assert {:msg "Initialization of network 'Net' might not establish the network invariant: Unread tokens might be left on channel e (#6)"} (C#[Net#e] - R#[Net#e]) == 0;
 }
 procedure Net##Add#anon$0#7()
-  modifies C, R, M, I, H, I#sub;
+  modifies C#, R#, M#, I#, H#, I#sub;
 {
   var Net#add: Actor;
   var Net#del: Actor;
@@ -205,64 +205,64 @@ procedure Net##Add#anon$0#7()
   var in2#j: int;
   assume (Net#add != Net#del) && (Net#add != Net#spl) && (Net#del != Net#spl);
   assume (Net#a != Net#b) && (Net#a != Net#c) && (Net#a != Net#d) && (Net#a != Net#e) && (Net#b != Net#c) && (Net#b != Net#d) && (Net#b != Net#e) && (Net#c != Net#d) && (Net#c != Net#e) && (Net#d != Net#e);
-  assume 0 <= I[Net#a];
-  assume I[Net#a] <= R[Net#a];
-  assume R[Net#a] <= C[Net#a];
-  assume 0 <= I[Net#b];
-  assume I[Net#b] <= R[Net#b];
-  assume R[Net#b] <= C[Net#b];
-  assume 0 <= I[Net#c];
-  assume I[Net#c] <= R[Net#c];
-  assume R[Net#c] <= C[Net#c];
-  assume 0 <= I[Net#d];
-  assume I[Net#d] <= R[Net#d];
-  assume R[Net#d] <= C[Net#d];
-  assume I[Net#d] == R[Net#d];
-  assume 0 <= I[Net#e];
-  assume I[Net#e] <= R[Net#e];
-  assume R[Net#e] <= C[Net#e];
-  assume (B[Net#a] == 1) && (B[Net#d] == 1);
-  I#sub[Net#a] := R[Net#a];
-  I#sub[Net#b] := R[Net#b];
-  I#sub[Net#c] := C[Net#c];
-  assume M[Net#b][0] == 0;
-  assume 0 <= M[Net#b][I[Net#b]];
-  assume I[Net#c] == I[Net#a];
-  assume I[Net#c] == I[Net#b];
-  assume I[Net#b] == I[Net#e];
-  assume I[Net#d] == I[Net#c];
-  assume I[Net#e] == I[Net#c];
-  assume 0 <= M[Net#a][I[Net#a]];
-  assume (C[Net#a] - I[Net#a]) <= 1;
-  assume R[Net#a] == C[Net#c];
-  assume R[Net#b] == C[Net#c];
+  assume 0 <= I#[Net#a];
+  assume I#[Net#a] <= R#[Net#a];
+  assume R#[Net#a] <= C#[Net#a];
+  assume 0 <= I#[Net#b];
+  assume I#[Net#b] <= R#[Net#b];
+  assume R#[Net#b] <= C#[Net#b];
+  assume 0 <= I#[Net#c];
+  assume I#[Net#c] <= R#[Net#c];
+  assume R#[Net#c] <= C#[Net#c];
+  assume 0 <= I#[Net#d];
+  assume I#[Net#d] <= R#[Net#d];
+  assume R#[Net#d] <= C#[Net#d];
+  assume I#[Net#d] == R#[Net#d];
+  assume 0 <= I#[Net#e];
+  assume I#[Net#e] <= R#[Net#e];
+  assume R#[Net#e] <= C#[Net#e];
+  assume (B#[Net#a] == 1) && (B#[Net#d] == 1);
+  I#sub[Net#a] := R#[Net#a];
+  I#sub[Net#b] := R#[Net#b];
+  I#sub[Net#c] := C#[Net#c];
+  assume M#[Net#b][0] == 0;
+  assume 0 <= M#[Net#b][I#[Net#b]];
+  assume I#[Net#c] == I#[Net#a];
+  assume I#[Net#c] == I#[Net#b];
+  assume I#[Net#b] == I#[Net#e];
+  assume I#[Net#d] == I#[Net#c];
+  assume I#[Net#e] == I#[Net#c];
+  assume 0 <= M#[Net#a][I#[Net#a]];
+  assume (C#[Net#a] - I#[Net#a]) <= 1;
+  assume R#[Net#a] == C#[Net#c];
+  assume R#[Net#b] == C#[Net#c];
   assume (forall idx$: int :: 
-    (0 <= idx$) && (idx$ < C[Net#c]) ==> (M[Net#c][idx$] == (M[Net#a][idx$] + M[Net#b][idx$]))
+    (0 <= idx$) && (idx$ < C#[Net#c]) ==> (M#[Net#c][idx$] == (M#[Net#a][idx$] + M#[Net#b][idx$]))
   );
-  assume R[Net#e] == (C[Net#b] - 1);
+  assume R#[Net#e] == (C#[Net#b] - 1);
   assume (forall idx$: int :: 
-    (1 <= idx$) && (idx$ < C[Net#b]) ==> (M[Net#b][idx$] == M[Net#e][idx$ - 1])
+    (1 <= idx$) && (idx$ < C#[Net#b]) ==> (M#[Net#b][idx$] == M#[Net#e][idx$ - 1])
   );
-  assume R[Net#c] == C[Net#d];
-  assume R[Net#c] == C[Net#e];
+  assume R#[Net#c] == C#[Net#d];
+  assume R#[Net#c] == C#[Net#e];
   assume (forall idx$: int :: 
-    (0 <= idx$) && (idx$ < C[Net#d]) ==> (M[Net#d][idx$] == M[Net#c][idx$])
+    (0 <= idx$) && (idx$ < C#[Net#d]) ==> (M#[Net#d][idx$] == M#[Net#c][idx$])
   );
   assume (forall idx$: int :: 
-    (0 <= idx$) && (idx$ < C[Net#e]) ==> (M[Net#e][idx$] == M[Net#c][idx$])
+    (0 <= idx$) && (idx$ < C#[Net#e]) ==> (M#[Net#e][idx$] == M#[Net#c][idx$])
   );
-  assume (1 <= (C[Net#a] - R[Net#a])) && (1 <= (C[Net#b] - R[Net#b]));
-  in1#i := M[Net#a][R[Net#a]];
-  R[Net#a] := R[Net#a] + 1;
-  in2#j := M[Net#b][R[Net#b]];
-  R[Net#b] := R[Net#b] + 1;
-  M[Net#c][C[Net#c]] := in1#i + in2#j;
-  C[Net#c] := C[Net#c] + 1;
-  assert {:msg "AddDelay.actor(24.15): Action at AddDelay.actor(2.3) ('anon$0') for actor instance 'add' might not preserve the channel invariant (#7)"} M[Net#b][0] == 0;
-  assert {:msg "AddDelay.actor(25.15): Action at AddDelay.actor(2.3) ('anon$0') for actor instance 'add' might not preserve the channel invariant (#8)"} 0 <= M[Net#b][I[Net#b]];
+  assume (1 <= (C#[Net#a] - R#[Net#a])) && (1 <= (C#[Net#b] - R#[Net#b]));
+  in1#i := M#[Net#a][R#[Net#a]];
+  R#[Net#a] := R#[Net#a] + 1;
+  in2#j := M#[Net#b][R#[Net#b]];
+  R#[Net#b] := R#[Net#b] + 1;
+  M#[Net#c][C#[Net#c]] := in1#i + in2#j;
+  C#[Net#c] := C#[Net#c] + 1;
+  assert {:msg "AddDelay.actor(24.15): Action at AddDelay.actor(2.3) ('anon$0') for actor instance 'add' might not preserve the channel invariant (#7)"} M#[Net#b][0] == 0;
+  assert {:msg "AddDelay.actor(25.15): Action at AddDelay.actor(2.3) ('anon$0') for actor instance 'add' might not preserve the channel invariant (#8)"} 0 <= M#[Net#b][I#[Net#b]];
 }
 procedure Net##Delay#anon$3#8()
-  modifies C, R, M, I, H, I#sub;
+  modifies C#, R#, M#, I#, H#, I#sub;
 {
   var Net#add: Actor;
   var Net#del: Actor;
@@ -275,61 +275,61 @@ procedure Net##Delay#anon$3#8()
   var in#i: int;
   assume (Net#add != Net#del) && (Net#add != Net#spl) && (Net#del != Net#spl);
   assume (Net#a != Net#b) && (Net#a != Net#c) && (Net#a != Net#d) && (Net#a != Net#e) && (Net#b != Net#c) && (Net#b != Net#d) && (Net#b != Net#e) && (Net#c != Net#d) && (Net#c != Net#e) && (Net#d != Net#e);
-  assume 0 <= I[Net#a];
-  assume I[Net#a] <= R[Net#a];
-  assume R[Net#a] <= C[Net#a];
-  assume 0 <= I[Net#b];
-  assume I[Net#b] <= R[Net#b];
-  assume R[Net#b] <= C[Net#b];
-  assume 0 <= I[Net#c];
-  assume I[Net#c] <= R[Net#c];
-  assume R[Net#c] <= C[Net#c];
-  assume 0 <= I[Net#d];
-  assume I[Net#d] <= R[Net#d];
-  assume R[Net#d] <= C[Net#d];
-  assume I[Net#d] == R[Net#d];
-  assume 0 <= I[Net#e];
-  assume I[Net#e] <= R[Net#e];
-  assume R[Net#e] <= C[Net#e];
-  assume (B[Net#a] == 1) && (B[Net#d] == 1);
-  I#sub[Net#e] := R[Net#e];
-  I#sub[Net#b] := C[Net#b];
-  assume M[Net#b][0] == 0;
-  assume 0 <= M[Net#b][I[Net#b]];
-  assume I[Net#c] == I[Net#a];
-  assume I[Net#c] == I[Net#b];
-  assume I[Net#b] == I[Net#e];
-  assume I[Net#d] == I[Net#c];
-  assume I[Net#e] == I[Net#c];
-  assume 0 <= M[Net#a][I[Net#a]];
-  assume (C[Net#a] - I[Net#a]) <= 1;
-  assume R[Net#a] == C[Net#c];
-  assume R[Net#b] == C[Net#c];
+  assume 0 <= I#[Net#a];
+  assume I#[Net#a] <= R#[Net#a];
+  assume R#[Net#a] <= C#[Net#a];
+  assume 0 <= I#[Net#b];
+  assume I#[Net#b] <= R#[Net#b];
+  assume R#[Net#b] <= C#[Net#b];
+  assume 0 <= I#[Net#c];
+  assume I#[Net#c] <= R#[Net#c];
+  assume R#[Net#c] <= C#[Net#c];
+  assume 0 <= I#[Net#d];
+  assume I#[Net#d] <= R#[Net#d];
+  assume R#[Net#d] <= C#[Net#d];
+  assume I#[Net#d] == R#[Net#d];
+  assume 0 <= I#[Net#e];
+  assume I#[Net#e] <= R#[Net#e];
+  assume R#[Net#e] <= C#[Net#e];
+  assume (B#[Net#a] == 1) && (B#[Net#d] == 1);
+  I#sub[Net#e] := R#[Net#e];
+  I#sub[Net#b] := C#[Net#b];
+  assume M#[Net#b][0] == 0;
+  assume 0 <= M#[Net#b][I#[Net#b]];
+  assume I#[Net#c] == I#[Net#a];
+  assume I#[Net#c] == I#[Net#b];
+  assume I#[Net#b] == I#[Net#e];
+  assume I#[Net#d] == I#[Net#c];
+  assume I#[Net#e] == I#[Net#c];
+  assume 0 <= M#[Net#a][I#[Net#a]];
+  assume (C#[Net#a] - I#[Net#a]) <= 1;
+  assume R#[Net#a] == C#[Net#c];
+  assume R#[Net#b] == C#[Net#c];
   assume (forall idx$: int :: 
-    (0 <= idx$) && (idx$ < C[Net#c]) ==> (M[Net#c][idx$] == (M[Net#a][idx$] + M[Net#b][idx$]))
+    (0 <= idx$) && (idx$ < C#[Net#c]) ==> (M#[Net#c][idx$] == (M#[Net#a][idx$] + M#[Net#b][idx$]))
   );
-  assume R[Net#e] == (C[Net#b] - 1);
+  assume R#[Net#e] == (C#[Net#b] - 1);
   assume (forall idx$: int :: 
-    (1 <= idx$) && (idx$ < C[Net#b]) ==> (M[Net#b][idx$] == M[Net#e][idx$ - 1])
+    (1 <= idx$) && (idx$ < C#[Net#b]) ==> (M#[Net#b][idx$] == M#[Net#e][idx$ - 1])
   );
-  assume R[Net#c] == C[Net#d];
-  assume R[Net#c] == C[Net#e];
+  assume R#[Net#c] == C#[Net#d];
+  assume R#[Net#c] == C#[Net#e];
   assume (forall idx$: int :: 
-    (0 <= idx$) && (idx$ < C[Net#d]) ==> (M[Net#d][idx$] == M[Net#c][idx$])
+    (0 <= idx$) && (idx$ < C#[Net#d]) ==> (M#[Net#d][idx$] == M#[Net#c][idx$])
   );
   assume (forall idx$: int :: 
-    (0 <= idx$) && (idx$ < C[Net#e]) ==> (M[Net#e][idx$] == M[Net#c][idx$])
+    (0 <= idx$) && (idx$ < C#[Net#e]) ==> (M#[Net#e][idx$] == M#[Net#c][idx$])
   );
-  assume 1 <= (C[Net#e] - R[Net#e]);
-  in#i := M[Net#e][R[Net#e]];
-  R[Net#e] := R[Net#e] + 1;
-  M[Net#b][C[Net#b]] := in#i;
-  C[Net#b] := C[Net#b] + 1;
-  assert {:msg "AddDelay.actor(24.15): Action at AddDelay.actor(11.3) ('anon$3') for actor instance 'del' might not preserve the channel invariant (#9)"} M[Net#b][0] == 0;
-  assert {:msg "AddDelay.actor(25.15): Action at AddDelay.actor(11.3) ('anon$3') for actor instance 'del' might not preserve the channel invariant (#10)"} 0 <= M[Net#b][I[Net#b]];
+  assume 1 <= (C#[Net#e] - R#[Net#e]);
+  in#i := M#[Net#e][R#[Net#e]];
+  R#[Net#e] := R#[Net#e] + 1;
+  M#[Net#b][C#[Net#b]] := in#i;
+  C#[Net#b] := C#[Net#b] + 1;
+  assert {:msg "AddDelay.actor(24.15): Action at AddDelay.actor(11.3) ('anon$3') for actor instance 'del' might not preserve the channel invariant (#9)"} M#[Net#b][0] == 0;
+  assert {:msg "AddDelay.actor(25.15): Action at AddDelay.actor(11.3) ('anon$3') for actor instance 'del' might not preserve the channel invariant (#10)"} 0 <= M#[Net#b][I#[Net#b]];
 }
 procedure Net##Split#anon$1#9()
-  modifies C, R, M, I, H, I#sub;
+  modifies C#, R#, M#, I#, H#, I#sub;
 {
   var Net#add: Actor;
   var Net#del: Actor;
@@ -342,64 +342,64 @@ procedure Net##Split#anon$1#9()
   var in#i: int;
   assume (Net#add != Net#del) && (Net#add != Net#spl) && (Net#del != Net#spl);
   assume (Net#a != Net#b) && (Net#a != Net#c) && (Net#a != Net#d) && (Net#a != Net#e) && (Net#b != Net#c) && (Net#b != Net#d) && (Net#b != Net#e) && (Net#c != Net#d) && (Net#c != Net#e) && (Net#d != Net#e);
-  assume 0 <= I[Net#a];
-  assume I[Net#a] <= R[Net#a];
-  assume R[Net#a] <= C[Net#a];
-  assume 0 <= I[Net#b];
-  assume I[Net#b] <= R[Net#b];
-  assume R[Net#b] <= C[Net#b];
-  assume 0 <= I[Net#c];
-  assume I[Net#c] <= R[Net#c];
-  assume R[Net#c] <= C[Net#c];
-  assume 0 <= I[Net#d];
-  assume I[Net#d] <= R[Net#d];
-  assume R[Net#d] <= C[Net#d];
-  assume I[Net#d] == R[Net#d];
-  assume 0 <= I[Net#e];
-  assume I[Net#e] <= R[Net#e];
-  assume R[Net#e] <= C[Net#e];
-  assume (B[Net#a] == 1) && (B[Net#d] == 1);
-  I#sub[Net#c] := R[Net#c];
-  I#sub[Net#d] := C[Net#d];
-  I#sub[Net#e] := C[Net#e];
-  assume M[Net#b][0] == 0;
-  assume 0 <= M[Net#b][I[Net#b]];
-  assume I[Net#c] == I[Net#a];
-  assume I[Net#c] == I[Net#b];
-  assume I[Net#b] == I[Net#e];
-  assume I[Net#d] == I[Net#c];
-  assume I[Net#e] == I[Net#c];
-  assume 0 <= M[Net#a][I[Net#a]];
-  assume (C[Net#a] - I[Net#a]) <= 1;
-  assume R[Net#a] == C[Net#c];
-  assume R[Net#b] == C[Net#c];
+  assume 0 <= I#[Net#a];
+  assume I#[Net#a] <= R#[Net#a];
+  assume R#[Net#a] <= C#[Net#a];
+  assume 0 <= I#[Net#b];
+  assume I#[Net#b] <= R#[Net#b];
+  assume R#[Net#b] <= C#[Net#b];
+  assume 0 <= I#[Net#c];
+  assume I#[Net#c] <= R#[Net#c];
+  assume R#[Net#c] <= C#[Net#c];
+  assume 0 <= I#[Net#d];
+  assume I#[Net#d] <= R#[Net#d];
+  assume R#[Net#d] <= C#[Net#d];
+  assume I#[Net#d] == R#[Net#d];
+  assume 0 <= I#[Net#e];
+  assume I#[Net#e] <= R#[Net#e];
+  assume R#[Net#e] <= C#[Net#e];
+  assume (B#[Net#a] == 1) && (B#[Net#d] == 1);
+  I#sub[Net#c] := R#[Net#c];
+  I#sub[Net#d] := C#[Net#d];
+  I#sub[Net#e] := C#[Net#e];
+  assume M#[Net#b][0] == 0;
+  assume 0 <= M#[Net#b][I#[Net#b]];
+  assume I#[Net#c] == I#[Net#a];
+  assume I#[Net#c] == I#[Net#b];
+  assume I#[Net#b] == I#[Net#e];
+  assume I#[Net#d] == I#[Net#c];
+  assume I#[Net#e] == I#[Net#c];
+  assume 0 <= M#[Net#a][I#[Net#a]];
+  assume (C#[Net#a] - I#[Net#a]) <= 1;
+  assume R#[Net#a] == C#[Net#c];
+  assume R#[Net#b] == C#[Net#c];
   assume (forall idx$: int :: 
-    (0 <= idx$) && (idx$ < C[Net#c]) ==> (M[Net#c][idx$] == (M[Net#a][idx$] + M[Net#b][idx$]))
+    (0 <= idx$) && (idx$ < C#[Net#c]) ==> (M#[Net#c][idx$] == (M#[Net#a][idx$] + M#[Net#b][idx$]))
   );
-  assume R[Net#e] == (C[Net#b] - 1);
+  assume R#[Net#e] == (C#[Net#b] - 1);
   assume (forall idx$: int :: 
-    (1 <= idx$) && (idx$ < C[Net#b]) ==> (M[Net#b][idx$] == M[Net#e][idx$ - 1])
+    (1 <= idx$) && (idx$ < C#[Net#b]) ==> (M#[Net#b][idx$] == M#[Net#e][idx$ - 1])
   );
-  assume R[Net#c] == C[Net#d];
-  assume R[Net#c] == C[Net#e];
+  assume R#[Net#c] == C#[Net#d];
+  assume R#[Net#c] == C#[Net#e];
   assume (forall idx$: int :: 
-    (0 <= idx$) && (idx$ < C[Net#d]) ==> (M[Net#d][idx$] == M[Net#c][idx$])
+    (0 <= idx$) && (idx$ < C#[Net#d]) ==> (M#[Net#d][idx$] == M#[Net#c][idx$])
   );
   assume (forall idx$: int :: 
-    (0 <= idx$) && (idx$ < C[Net#e]) ==> (M[Net#e][idx$] == M[Net#c][idx$])
+    (0 <= idx$) && (idx$ < C#[Net#e]) ==> (M#[Net#e][idx$] == M#[Net#c][idx$])
   );
-  assume 1 <= (C[Net#c] - R[Net#c]);
-  in#i := M[Net#c][R[Net#c]];
-  R[Net#c] := R[Net#c] + 1;
-  M[Net#d][C[Net#d]] := in#i;
-  C[Net#d] := C[Net#d] + 1;
-  M[Net#e][C[Net#e]] := in#i;
-  C[Net#e] := C[Net#e] + 1;
-  assert {:msg "AddDelay.actor(24.15): Action at AddDelay.actor(6.3) ('anon$1') for actor instance 'spl' might not preserve the channel invariant (#11)"} M[Net#b][0] == 0;
-  assert {:msg "AddDelay.actor(25.15): Action at AddDelay.actor(6.3) ('anon$1') for actor instance 'spl' might not preserve the channel invariant (#12)"} 0 <= M[Net#b][I[Net#b]];
+  assume 1 <= (C#[Net#c] - R#[Net#c]);
+  in#i := M#[Net#c][R#[Net#c]];
+  R#[Net#c] := R#[Net#c] + 1;
+  M#[Net#d][C#[Net#d]] := in#i;
+  C#[Net#d] := C#[Net#d] + 1;
+  M#[Net#e][C#[Net#e]] := in#i;
+  C#[Net#e] := C#[Net#e] + 1;
+  assert {:msg "AddDelay.actor(24.15): Action at AddDelay.actor(6.3) ('anon$1') for actor instance 'spl' might not preserve the channel invariant (#11)"} M#[Net#b][0] == 0;
+  assert {:msg "AddDelay.actor(25.15): Action at AddDelay.actor(6.3) ('anon$1') for actor instance 'spl' might not preserve the channel invariant (#12)"} 0 <= M#[Net#b][I#[Net#b]];
 }
 procedure Net#anon$4#input#in#10()
-  modifies C, R, M, I, H, I#sub;
+  modifies C#, R#, M#, I#, H#, I#sub;
 {
   var Net#add: Actor;
   var Net#del: Actor;
@@ -411,58 +411,58 @@ procedure Net#anon$4#input#in#10()
   var Net#e: Chan (int);
   assume (Net#add != Net#del) && (Net#add != Net#spl) && (Net#del != Net#spl);
   assume (Net#a != Net#b) && (Net#a != Net#c) && (Net#a != Net#d) && (Net#a != Net#e) && (Net#b != Net#c) && (Net#b != Net#d) && (Net#b != Net#e) && (Net#c != Net#d) && (Net#c != Net#e) && (Net#d != Net#e);
-  assume 0 <= I[Net#a];
-  assume I[Net#a] <= R[Net#a];
-  assume R[Net#a] <= C[Net#a];
-  assume 0 <= I[Net#b];
-  assume I[Net#b] <= R[Net#b];
-  assume R[Net#b] <= C[Net#b];
-  assume 0 <= I[Net#c];
-  assume I[Net#c] <= R[Net#c];
-  assume R[Net#c] <= C[Net#c];
-  assume 0 <= I[Net#d];
-  assume I[Net#d] <= R[Net#d];
-  assume R[Net#d] <= C[Net#d];
-  assume I[Net#d] == R[Net#d];
-  assume 0 <= I[Net#e];
-  assume I[Net#e] <= R[Net#e];
-  assume R[Net#e] <= C[Net#e];
-  assume (B[Net#a] == 1) && (B[Net#d] == 1);
-  assume (B[Net#a] == 1) && (B[Net#d] == 1);
-  assume (C[Net#a] - I[Net#a]) < 1;
-  assume M[Net#b][0] == 0;
-  assume 0 <= M[Net#b][I[Net#b]];
-  assume I[Net#c] == I[Net#a];
-  assume I[Net#c] == I[Net#b];
-  assume I[Net#b] == I[Net#e];
-  assume I[Net#d] == I[Net#c];
-  assume I[Net#e] == I[Net#c];
-  assume 0 <= M[Net#a][I[Net#a]];
-  assume (C[Net#a] - I[Net#a]) <= 1;
-  assume R[Net#a] == C[Net#c];
-  assume R[Net#b] == C[Net#c];
+  assume 0 <= I#[Net#a];
+  assume I#[Net#a] <= R#[Net#a];
+  assume R#[Net#a] <= C#[Net#a];
+  assume 0 <= I#[Net#b];
+  assume I#[Net#b] <= R#[Net#b];
+  assume R#[Net#b] <= C#[Net#b];
+  assume 0 <= I#[Net#c];
+  assume I#[Net#c] <= R#[Net#c];
+  assume R#[Net#c] <= C#[Net#c];
+  assume 0 <= I#[Net#d];
+  assume I#[Net#d] <= R#[Net#d];
+  assume R#[Net#d] <= C#[Net#d];
+  assume I#[Net#d] == R#[Net#d];
+  assume 0 <= I#[Net#e];
+  assume I#[Net#e] <= R#[Net#e];
+  assume R#[Net#e] <= C#[Net#e];
+  assume (B#[Net#a] == 1) && (B#[Net#d] == 1);
+  assume (B#[Net#a] == 1) && (B#[Net#d] == 1);
+  assume (C#[Net#a] - I#[Net#a]) < 1;
+  assume M#[Net#b][0] == 0;
+  assume 0 <= M#[Net#b][I#[Net#b]];
+  assume I#[Net#c] == I#[Net#a];
+  assume I#[Net#c] == I#[Net#b];
+  assume I#[Net#b] == I#[Net#e];
+  assume I#[Net#d] == I#[Net#c];
+  assume I#[Net#e] == I#[Net#c];
+  assume 0 <= M#[Net#a][I#[Net#a]];
+  assume (C#[Net#a] - I#[Net#a]) <= 1;
+  assume R#[Net#a] == C#[Net#c];
+  assume R#[Net#b] == C#[Net#c];
   assume (forall idx$: int :: 
-    (0 <= idx$) && (idx$ < C[Net#c]) ==> (M[Net#c][idx$] == (M[Net#a][idx$] + M[Net#b][idx$]))
+    (0 <= idx$) && (idx$ < C#[Net#c]) ==> (M#[Net#c][idx$] == (M#[Net#a][idx$] + M#[Net#b][idx$]))
   );
-  assume R[Net#e] == (C[Net#b] - 1);
+  assume R#[Net#e] == (C#[Net#b] - 1);
   assume (forall idx$: int :: 
-    (1 <= idx$) && (idx$ < C[Net#b]) ==> (M[Net#b][idx$] == M[Net#e][idx$ - 1])
+    (1 <= idx$) && (idx$ < C#[Net#b]) ==> (M#[Net#b][idx$] == M#[Net#e][idx$ - 1])
   );
-  assume R[Net#c] == C[Net#d];
-  assume R[Net#c] == C[Net#e];
+  assume R#[Net#c] == C#[Net#d];
+  assume R#[Net#c] == C#[Net#e];
   assume (forall idx$: int :: 
-    (0 <= idx$) && (idx$ < C[Net#d]) ==> (M[Net#d][idx$] == M[Net#c][idx$])
+    (0 <= idx$) && (idx$ < C#[Net#d]) ==> (M#[Net#d][idx$] == M#[Net#c][idx$])
   );
   assume (forall idx$: int :: 
-    (0 <= idx$) && (idx$ < C[Net#e]) ==> (M[Net#e][idx$] == M[Net#c][idx$])
+    (0 <= idx$) && (idx$ < C#[Net#e]) ==> (M#[Net#e][idx$] == M#[Net#c][idx$])
   );
-  C[Net#a] := C[Net#a] + 1;
-  assume 0 <= M[Net#a][I[Net#a]];
-  assert {:msg "AddDelay.actor(24.15): Channel invariant might be falsified by network input (#13)"} M[Net#b][0] == 0;
-  assert {:msg "AddDelay.actor(25.15): Channel invariant might be falsified by network input (#14)"} 0 <= M[Net#b][I[Net#b]];
+  C#[Net#a] := C#[Net#a] + 1;
+  assume 0 <= M#[Net#a][I#[Net#a]];
+  assert {:msg "AddDelay.actor(24.15): Channel invariant might be falsified by network input (#13)"} M#[Net#b][0] == 0;
+  assert {:msg "AddDelay.actor(25.15): Channel invariant might be falsified by network input (#14)"} 0 <= M#[Net#b][I#[Net#b]];
 }
 procedure Net#anon$4#exit#11()
-  modifies C, R, M, I, H, I#sub;
+  modifies C#, R#, M#, I#, H#, I#sub;
 {
   var Net#add: Actor;
   var Net#del: Actor;
@@ -474,66 +474,66 @@ procedure Net#anon$4#exit#11()
   var Net#e: Chan (int);
   assume (Net#add != Net#del) && (Net#add != Net#spl) && (Net#del != Net#spl);
   assume (Net#a != Net#b) && (Net#a != Net#c) && (Net#a != Net#d) && (Net#a != Net#e) && (Net#b != Net#c) && (Net#b != Net#d) && (Net#b != Net#e) && (Net#c != Net#d) && (Net#c != Net#e) && (Net#d != Net#e);
-  assume 0 <= I[Net#a];
-  assume I[Net#a] <= R[Net#a];
-  assume R[Net#a] <= C[Net#a];
-  assume 0 <= I[Net#b];
-  assume I[Net#b] <= R[Net#b];
-  assume R[Net#b] <= C[Net#b];
-  assume 0 <= I[Net#c];
-  assume I[Net#c] <= R[Net#c];
-  assume R[Net#c] <= C[Net#c];
-  assume 0 <= I[Net#d];
-  assume I[Net#d] <= R[Net#d];
-  assume R[Net#d] <= C[Net#d];
-  assume I[Net#d] == R[Net#d];
-  assume 0 <= I[Net#e];
-  assume I[Net#e] <= R[Net#e];
-  assume R[Net#e] <= C[Net#e];
-  assume (B[Net#a] == 1) && (B[Net#d] == 1);
-  assume (B[Net#a] == 1) && (B[Net#d] == 1);
-  assume M[Net#b][0] == 0;
-  assume 0 <= M[Net#b][I[Net#b]];
-  assume I[Net#c] == I[Net#a];
-  assume I[Net#c] == I[Net#b];
-  assume I[Net#b] == I[Net#e];
-  assume I[Net#d] == I[Net#c];
-  assume I[Net#e] == I[Net#c];
-  assume 0 <= M[Net#a][I[Net#a]];
-  assume (C[Net#a] - I[Net#a]) <= 1;
-  assume R[Net#a] == C[Net#c];
-  assume R[Net#b] == C[Net#c];
+  assume 0 <= I#[Net#a];
+  assume I#[Net#a] <= R#[Net#a];
+  assume R#[Net#a] <= C#[Net#a];
+  assume 0 <= I#[Net#b];
+  assume I#[Net#b] <= R#[Net#b];
+  assume R#[Net#b] <= C#[Net#b];
+  assume 0 <= I#[Net#c];
+  assume I#[Net#c] <= R#[Net#c];
+  assume R#[Net#c] <= C#[Net#c];
+  assume 0 <= I#[Net#d];
+  assume I#[Net#d] <= R#[Net#d];
+  assume R#[Net#d] <= C#[Net#d];
+  assume I#[Net#d] == R#[Net#d];
+  assume 0 <= I#[Net#e];
+  assume I#[Net#e] <= R#[Net#e];
+  assume R#[Net#e] <= C#[Net#e];
+  assume (B#[Net#a] == 1) && (B#[Net#d] == 1);
+  assume (B#[Net#a] == 1) && (B#[Net#d] == 1);
+  assume M#[Net#b][0] == 0;
+  assume 0 <= M#[Net#b][I#[Net#b]];
+  assume I#[Net#c] == I#[Net#a];
+  assume I#[Net#c] == I#[Net#b];
+  assume I#[Net#b] == I#[Net#e];
+  assume I#[Net#d] == I#[Net#c];
+  assume I#[Net#e] == I#[Net#c];
+  assume 0 <= M#[Net#a][I#[Net#a]];
+  assume (C#[Net#a] - I#[Net#a]) <= 1;
+  assume R#[Net#a] == C#[Net#c];
+  assume R#[Net#b] == C#[Net#c];
   assume (forall idx$: int :: 
-    (0 <= idx$) && (idx$ < C[Net#c]) ==> (M[Net#c][idx$] == (M[Net#a][idx$] + M[Net#b][idx$]))
+    (0 <= idx$) && (idx$ < C#[Net#c]) ==> (M#[Net#c][idx$] == (M#[Net#a][idx$] + M#[Net#b][idx$]))
   );
-  assume R[Net#e] == (C[Net#b] - 1);
+  assume R#[Net#e] == (C#[Net#b] - 1);
   assume (forall idx$: int :: 
-    (1 <= idx$) && (idx$ < C[Net#b]) ==> (M[Net#b][idx$] == M[Net#e][idx$ - 1])
+    (1 <= idx$) && (idx$ < C#[Net#b]) ==> (M#[Net#b][idx$] == M#[Net#e][idx$ - 1])
   );
-  assume R[Net#c] == C[Net#d];
-  assume R[Net#c] == C[Net#e];
+  assume R#[Net#c] == C#[Net#d];
+  assume R#[Net#c] == C#[Net#e];
   assume (forall idx$: int :: 
-    (0 <= idx$) && (idx$ < C[Net#d]) ==> (M[Net#d][idx$] == M[Net#c][idx$])
+    (0 <= idx$) && (idx$ < C#[Net#d]) ==> (M#[Net#d][idx$] == M#[Net#c][idx$])
   );
   assume (forall idx$: int :: 
-    (0 <= idx$) && (idx$ < C[Net#e]) ==> (M[Net#e][idx$] == M[Net#c][idx$])
+    (0 <= idx$) && (idx$ < C#[Net#e]) ==> (M#[Net#e][idx$] == M#[Net#c][idx$])
   );
-  assume (C[Net#a] - I[Net#a]) == 1;
-  assume 0 <= M[Net#a][I[Net#a]];
-  assume !((1 <= (C[Net#a] - R[Net#a])) && (1 <= (C[Net#b] - R[Net#b])));
-  assume !(1 <= (C[Net#e] - R[Net#e]));
-  assume !(1 <= (C[Net#c] - R[Net#c]));
-  assert {:msg "AddDelay.actor(16.3): The correct number of tokens might not be produced on output 'out' (#15)"} (C[Net#d] - I[Net#d]) == 1;
-  assert {:msg "AddDelay.actor(18.13): Network action postcondition might not hold (#16)"} M[Net#d][0] == M[Net#a][0];
-  assert {:msg "AddDelay.actor(19.13): Network action postcondition might not hold (#17)"} M[Net#d][I[Net#d]] >= M[Net#a][I[Net#a]];
-  assert {:msg "AddDelay.actor(20.13): Network action postcondition might not hold (#18)"} (0 < I[Net#d]) ==> (M[Net#d][I[Net#d]] == (M[Net#d][I[Net#d] - 1] + M[Net#a][I[Net#a]]));
-  R[Net#d] := R[Net#d] + 1;
-  I := R;
-  assert {:msg "AddDelay.actor(24.15): The network might not preserve the channel invariant (#19)"} M[Net#b][0] == 0;
-  assert {:msg "AddDelay.actor(25.15): The network might not preserve the channel invariant (#20)"} 0 <= M[Net#b][I[Net#b]];
-  assert {:msg "AddDelay.actor(23.13): The network might not preserve the network invariant (#21)"} (C[Net#b] - R[Net#b]) == 1;
-  assert {:msg "The network might not preserve the network invariant: Unread tokens might be left on channel a (#22)"} (C[Net#a] - R[Net#a]) == 0;
-  assert {:msg "The network might not preserve the network invariant: Unread tokens might be left on channel c (#23)"} (C[Net#c] - R[Net#c]) == 0;
-  assert {:msg "The network might not preserve the network invariant: Unread tokens might be left on channel d (#24)"} (C[Net#d] - R[Net#d]) == 0;
-  assert {:msg "The network might not preserve the network invariant: Unread tokens might be left on channel e (#25)"} (C[Net#e] - R[Net#e]) == 0;
+  assume (C#[Net#a] - I#[Net#a]) == 1;
+  assume 0 <= M#[Net#a][I#[Net#a]];
+  assume !((1 <= (C#[Net#a] - R#[Net#a])) && (1 <= (C#[Net#b] - R#[Net#b])));
+  assume !(1 <= (C#[Net#e] - R#[Net#e]));
+  assume !(1 <= (C#[Net#c] - R#[Net#c]));
+  assert {:msg "AddDelay.actor(16.3): The correct number of tokens might not be produced on output 'out' (#15)"} (C#[Net#d] - I#[Net#d]) == 1;
+  assert {:msg "AddDelay.actor(18.13): Network action postcondition might not hold (#16)"} M#[Net#d][0] == M#[Net#a][0];
+  assert {:msg "AddDelay.actor(19.13): Network action postcondition might not hold (#17)"} M#[Net#d][I#[Net#d]] >= M#[Net#a][I#[Net#a]];
+  assert {:msg "AddDelay.actor(20.13): Network action postcondition might not hold (#18)"} (0 < I#[Net#d]) ==> (M#[Net#d][I#[Net#d]] == (M#[Net#d][I#[Net#d] - 1] + M#[Net#a][I#[Net#a]]));
+  R#[Net#d] := R#[Net#d] + 1;
+  I# := R#;
+  assert {:msg "AddDelay.actor(24.15): The network might not preserve the channel invariant (#19)"} M#[Net#b][0] == 0;
+  assert {:msg "AddDelay.actor(25.15): The network might not preserve the channel invariant (#20)"} 0 <= M#[Net#b][I#[Net#b]];
+  assert {:msg "AddDelay.actor(23.13): The network might not preserve the network invariant (#21)"} (C#[Net#b] - R#[Net#b]) == 1;
+  assert {:msg "The network might not preserve the network invariant: Unread tokens might be left on channel a (#22)"} (C#[Net#a] - R#[Net#a]) == 0;
+  assert {:msg "The network might not preserve the network invariant: Unread tokens might be left on channel c (#23)"} (C#[Net#c] - R#[Net#c]) == 0;
+  assert {:msg "The network might not preserve the network invariant: Unread tokens might be left on channel d (#24)"} (C#[Net#d] - R#[Net#d]) == 0;
+  assert {:msg "The network might not preserve the network invariant: Unread tokens might be left on channel e (#25)"} (C#[Net#e] - R#[Net#e]) == 0;
 }
