tests/zigbee/headerAdd.cal.bpl
@@ -11,15 +11,15 @@ type Obj = <a>[Field a]a;
 type HType = [Ref]Obj;
 type ModeType = [Actor]int;
 
-var M: MType;
-var C: CType;
-var R: CType;
-var I: CType;
-var B: CType;
-var Mode: ModeType;
+var M#: MType;
+var C#: CType;
+var R#: CType;
+var I#: CType;
+var B#: CType;
+var Mode#: ModeType;
 var I#sub: CType;
 
-var H: HType;
+var H#: HType;
 
 const unique this#: Actor;
 
@@ -48,9 +48,12 @@ axiom (
 function {:bvbuiltin "bvand"} AT#BvAnd8(a: bv8, b: bv8): bv8;
 function {:bvbuiltin "bvor"} AT#BvOr8(a: bv8, b: bv8): bv8;
 function {:bvbuiltin "bvnot"} AT#BvNot8(a: bv8): bv8;
+function {:bvbuiltin "bvneg"} AT#BvNeg8(a: bv8): bv8;
 function {:bvbuiltin "bvadd"} AT#BvAdd8(a: bv8, b: bv8): bv8;
 function {:bvbuiltin "bvsub"} AT#BvSub8(a: bv8, b: bv8): bv8;
 function {:bvbuiltin "bvmul"} AT#BvMul8(a: bv8, b: bv8): bv8;
+function {:bvbuiltin "bvsdiv"} AT#BvSdiv8(a: bv8, b: bv8): bv8;
+function {:bvbuiltin "bvudiv"} AT#BvUdiv8(a: bv8, b: bv8): bv8;
 function {:bvbuiltin "bvshl"} AT#BvShl8(bv8,bv8): bv8;
 function {:bvbuiltin "bvlshr"} AT#BvLshr8(bv8,bv8): bv8;
 function {:bvbuiltin "bvashr"} AT#BvAshr8(bv8,bv8): bv8;
@@ -63,15 +66,17 @@ function {:bvbuiltin "bvslt"} AT#BvSlt8(a: bv8, b: bv8): bool;
 function {:bvbuiltin "bvsge"} AT#BvSge8(a: bv8, b: bv8): bool;
 function {:bvbuiltin "bvsgt"} AT#BvSgt8(a: bv8, b: bv8): bool;
 function AT#BvXor8(a: bv8, b: bv8): bv8;
+function AT#BvAbs8(a: bv8): bv8;
 
 axiom (forall a,b: bv8 :: AT#BvXor8(a,b) == AT#BvAnd8(AT#BvOr8(a,b), AT#BvNot8(AT#BvAnd8(a,b))) );
+axiom (forall a,b: bv8 :: AT#BvAbs8(a) == (if AT#BvSle8(0bv8,a) then a else AT#BvNeg8(a)) );
 
 // ---------------------------------------------------------------
 // -- End of prelude ---------------------------------------------
 // ---------------------------------------------------------------
 
 procedure headerAdd#init#0()
-  modifies C, R, M, I, H, I#sub;
+  modifies C#, R#, M#, I#, H#, I#sub;
 {
   var pl_bits: Chan (bv8);
   var data: Chan (bv8);
@@ -84,9 +89,9 @@ procedure headerAdd#init#0()
   var St: int;
   assume (pl_bits != data) && (pl_bits != len) && (data != len);
   assume HEADER_LEN == 5;
-  assume (I[pl_bits] == 0) && (R[pl_bits] == 0) && (C[pl_bits] == 0);
-  assume (I[data] == 0) && (R[data] == 0) && (C[data] == 0);
-  assume (I[len] == 0) && (R[len] == 0) && (C[len] == 0);
+  assume (I#[pl_bits] == 0) && (R#[pl_bits] == 0) && (C#[pl_bits] == 0);
+  assume (I#[data] == 0) && (R#[data] == 0) && (C#[data] == 0);
+  assume (I#[len] == 0) && (R#[len] == 0) && (C#[len] == 0);
   octet_index := 0bv8;
   octet_count := 14bv8;
   St := 0;
@@ -98,7 +103,7 @@ procedure headerAdd#init#0()
   assert {:msg "headerAdd.cal(31.12): Initialization might not establish the invariant (#5)"} (0 <= St) && (St <= 2);
 }
 procedure headerAdd#get_data_len#1()
-  modifies C, R, M, I, H, I#sub;
+  modifies C#, R#, M#, I#, H#, I#sub;
 {
   var pl_bits: Chan (bv8);
   var data: Chan (bv8);
@@ -112,25 +117,25 @@ procedure headerAdd#get_data_len#1()
   var pl_bits#0: bv8;
   assume (pl_bits != data) && (pl_bits != len) && (data != len);
   assume HEADER_LEN == 5;
-  assume (0 <= I[pl_bits]) && (I[pl_bits] <= R[pl_bits]) && (R[pl_bits] <= C[pl_bits]);
-  assume (0 <= I[data]) && (I[data] <= R[data]) && (R[data] <= C[data]);
-  assume (0 <= I[len]) && (I[len] <= R[len]) && (R[len] <= C[len]);
+  assume (0 <= I#[pl_bits]) && (I#[pl_bits] <= R#[pl_bits]) && (R#[pl_bits] <= C#[pl_bits]);
+  assume (0 <= I#[data]) && (I#[data] <= R#[data]) && (R#[data] <= C#[data]);
+  assume (0 <= I#[len]) && (I#[len] <= R#[len]) && (R#[len] <= C#[len]);
   assume AT#BvUle8(0bv8, octet_index);
   assume AT#BvUle8(octet_index, octet_count);
   assume octet_count == 14bv8;
   assume (St == 1) ==> AT#BvUle8(octet_index, 5bv8);
   assume (St == 2) ==> AT#BvUlt8(5bv8, octet_index);
   assume (0 <= St) && (St <= 2);
-  assume 1 <= (C[pl_bits] - R[pl_bits]);
-  pl_bits#0 := M[pl_bits][R[pl_bits]];
-  R[pl_bits] := R[pl_bits] + 1;
+  assume 1 <= (C#[pl_bits] - R#[pl_bits]);
+  pl_bits#0 := M#[pl_bits][R#[pl_bits]];
+  R#[pl_bits] := R#[pl_bits] + 1;
   assume pl_bits#0 == 8bv8;
   assume St == 0;
   octet_index := 0bv8;
   octet_count := AT#BvAdd8(AT#BvAdd8(pl_bits#0, 5bv8), 1bv8);
   St := 1;
-  M[len][C[len]] := octet_count;
-  C[len] := C[len] + 1;
+  M#[len][C#[len]] := octet_count;
+  C#[len] := C#[len] + 1;
   assert {:msg "headerAdd.cal(25.12): Action 'get_data_len' at headerAdd.cal(46.2) might not preserve the invariant (#6)"} AT#BvUle8(0bv8, octet_index);
   assert {:msg "headerAdd.cal(26.12): Action 'get_data_len' at headerAdd.cal(46.2) might not preserve the invariant (#7)"} AT#BvUle8(octet_index, octet_count);
   assert {:msg "headerAdd.cal(27.12): Action 'get_data_len' at headerAdd.cal(46.2) might not preserve the invariant (#8)"} octet_count == 14bv8;
@@ -139,7 +144,7 @@ procedure headerAdd#get_data_len#1()
   assert {:msg "headerAdd.cal(31.12): Action 'get_data_len' at headerAdd.cal(46.2) might not preserve the invariant (#11)"} (0 <= St) && (St <= 2);
 }
 procedure headerAdd#send_header#2()
-  modifies C, R, M, I, H, I#sub;
+  modifies C#, R#, M#, I#, H#, I#sub;
 {
   var pl_bits: Chan (bv8);
   var data: Chan (bv8);
@@ -153,9 +158,9 @@ procedure headerAdd#send_header#2()
   var pl_bits#0: bv8;
   assume (pl_bits != data) && (pl_bits != len) && (data != len);
   assume HEADER_LEN == 5;
-  assume (0 <= I[pl_bits]) && (I[pl_bits] <= R[pl_bits]) && (R[pl_bits] <= C[pl_bits]);
-  assume (0 <= I[data]) && (I[data] <= R[data]) && (R[data] <= C[data]);
-  assume (0 <= I[len]) && (I[len] <= R[len]) && (R[len] <= C[len]);
+  assume (0 <= I#[pl_bits]) && (I#[pl_bits] <= R#[pl_bits]) && (R#[pl_bits] <= C#[pl_bits]);
+  assume (0 <= I#[data]) && (I#[data] <= R#[data]) && (R#[data] <= C#[data]);
+  assume (0 <= I#[len]) && (I#[len] <= R#[len]) && (R#[len] <= C#[len]);
   assume AT#BvUle8(0bv8, octet_index);
   assume AT#BvUle8(octet_index, octet_count);
   assume octet_count == 14bv8;
@@ -167,8 +172,8 @@ procedure headerAdd#send_header#2()
   data_out := Map#Select(Header, octet_index);
   octet_index := AT#BvAdd8(octet_index, 1bv8);
   St := 1;
-  M[data][C[data]] := data_out;
-  C[data] := C[data] + 1;
+  M#[data][C#[data]] := data_out;
+  C#[data] := C#[data] + 1;
   assert {:msg "headerAdd.cal(25.12): Action 'send_header' at headerAdd.cal(57.2) might not preserve the invariant (#12)"} AT#BvUle8(0bv8, octet_index);
   assert {:msg "headerAdd.cal(26.12): Action 'send_header' at headerAdd.cal(57.2) might not preserve the invariant (#13)"} AT#BvUle8(octet_index, octet_count);
   assert {:msg "headerAdd.cal(27.12): Action 'send_header' at headerAdd.cal(57.2) might not preserve the invariant (#14)"} octet_count == 14bv8;
@@ -177,7 +182,7 @@ procedure headerAdd#send_header#2()
   assert {:msg "headerAdd.cal(31.12): Action 'send_header' at headerAdd.cal(57.2) might not preserve the invariant (#17)"} (0 <= St) && (St <= 2);
 }
 procedure headerAdd#send_length#3()
-  modifies C, R, M, I, H, I#sub;
+  modifies C#, R#, M#, I#, H#, I#sub;
 {
   var pl_bits: Chan (bv8);
   var data: Chan (bv8);
@@ -191,9 +196,9 @@ procedure headerAdd#send_length#3()
   var pl_bits#0: bv8;
   assume (pl_bits != data) && (pl_bits != len) && (data != len);
   assume HEADER_LEN == 5;
-  assume (0 <= I[pl_bits]) && (I[pl_bits] <= R[pl_bits]) && (R[pl_bits] <= C[pl_bits]);
-  assume (0 <= I[data]) && (I[data] <= R[data]) && (R[data] <= C[data]);
-  assume (0 <= I[len]) && (I[len] <= R[len]) && (R[len] <= C[len]);
+  assume (0 <= I#[pl_bits]) && (I#[pl_bits] <= R#[pl_bits]) && (R#[pl_bits] <= C#[pl_bits]);
+  assume (0 <= I#[data]) && (I#[data] <= R#[data]) && (R#[data] <= C#[data]);
+  assume (0 <= I#[len]) && (I#[len] <= R#[len]) && (R#[len] <= C#[len]);
   assume AT#BvUle8(0bv8, octet_index);
   assume AT#BvUle8(octet_index, octet_count);
   assume octet_count == 14bv8;
@@ -205,8 +210,8 @@ procedure headerAdd#send_length#3()
   assume (octet_index == 5bv8) && (St == 1);
   octet_index := AT#BvAdd8(octet_index, 1bv8);
   St := 2;
-  M[data][C[data]] := AT#BvSub8(AT#BvSub8(octet_count, 5bv8), 1bv8);
-  C[data] := C[data] + 1;
+  M#[data][C#[data]] := AT#BvSub8(AT#BvSub8(octet_count, 5bv8), 1bv8);
+  C#[data] := C#[data] + 1;
   assert {:msg "headerAdd.cal(25.12): Action 'send_length' at headerAdd.cal(69.2) might not preserve the invariant (#18)"} AT#BvUle8(0bv8, octet_index);
   assert {:msg "headerAdd.cal(26.12): Action 'send_length' at headerAdd.cal(69.2) might not preserve the invariant (#19)"} AT#BvUle8(octet_index, octet_count);
   assert {:msg "headerAdd.cal(27.12): Action 'send_length' at headerAdd.cal(69.2) might not preserve the invariant (#20)"} octet_count == 14bv8;
@@ -215,7 +220,7 @@ procedure headerAdd#send_length#3()
   assert {:msg "headerAdd.cal(31.12): Action 'send_length' at headerAdd.cal(69.2) might not preserve the invariant (#23)"} (0 <= St) && (St <= 2);
 }
 procedure headerAdd#send_payload_octet#4()
-  modifies C, R, M, I, H, I#sub;
+  modifies C#, R#, M#, I#, H#, I#sub;
 {
   var pl_bits: Chan (bv8);
   var data: Chan (bv8);
@@ -229,23 +234,23 @@ procedure headerAdd#send_payload_octet#4()
   var pl_bits#0: bv8;
   assume (pl_bits != data) && (pl_bits != len) && (data != len);
   assume HEADER_LEN == 5;
-  assume (0 <= I[pl_bits]) && (I[pl_bits] <= R[pl_bits]) && (R[pl_bits] <= C[pl_bits]);
-  assume (0 <= I[data]) && (I[data] <= R[data]) && (R[data] <= C[data]);
-  assume (0 <= I[len]) && (I[len] <= R[len]) && (R[len] <= C[len]);
+  assume (0 <= I#[pl_bits]) && (I#[pl_bits] <= R#[pl_bits]) && (R#[pl_bits] <= C#[pl_bits]);
+  assume (0 <= I#[data]) && (I#[data] <= R#[data]) && (R#[data] <= C#[data]);
+  assume (0 <= I#[len]) && (I#[len] <= R#[len]) && (R#[len] <= C#[len]);
   assume AT#BvUle8(0bv8, octet_index);
   assume AT#BvUle8(octet_index, octet_count);
   assume octet_count == 14bv8;
   assume (St == 1) ==> AT#BvUle8(octet_index, 5bv8);
   assume (St == 2) ==> AT#BvUlt8(5bv8, octet_index);
   assume (0 <= St) && (St <= 2);
-  assume 1 <= (C[pl_bits] - R[pl_bits]);
-  pl_bits#0 := M[pl_bits][R[pl_bits]];
-  R[pl_bits] := R[pl_bits] + 1;
+  assume 1 <= (C#[pl_bits] - R#[pl_bits]);
+  pl_bits#0 := M#[pl_bits][R#[pl_bits]];
+  R#[pl_bits] := R#[pl_bits] + 1;
   assume AT#BvUlt8(octet_index, octet_count) && (St == 2);
   octet_index := AT#BvAdd8(octet_index, 1bv8);
   St := 2;
-  M[data][C[data]] := pl_bits#0;
-  C[data] := C[data] + 1;
+  M#[data][C#[data]] := pl_bits#0;
+  C#[data] := C#[data] + 1;
   assert {:msg "headerAdd.cal(25.12): Action 'send_payload_octet' at headerAdd.cal(80.2) might not preserve the invariant (#24)"} AT#BvUle8(0bv8, octet_index);
   assert {:msg "headerAdd.cal(26.12): Action 'send_payload_octet' at headerAdd.cal(80.2) might not preserve the invariant (#25)"} AT#BvUle8(octet_index, octet_count);
   assert {:msg "headerAdd.cal(27.12): Action 'send_payload_octet' at headerAdd.cal(80.2) might not preserve the invariant (#26)"} octet_count == 14bv8;
@@ -254,7 +259,7 @@ procedure headerAdd#send_payload_octet#4()
   assert {:msg "headerAdd.cal(31.12): Action 'send_payload_octet' at headerAdd.cal(80.2) might not preserve the invariant (#29)"} (0 <= St) && (St <= 2);
 }
 procedure headerAdd#done#5()
-  modifies C, R, M, I, H, I#sub;
+  modifies C#, R#, M#, I#, H#, I#sub;
 {
   var pl_bits: Chan (bv8);
   var data: Chan (bv8);
@@ -268,9 +273,9 @@ procedure headerAdd#done#5()
   var pl_bits#0: bv8;
   assume (pl_bits != data) && (pl_bits != len) && (data != len);
   assume HEADER_LEN == 5;
-  assume (0 <= I[pl_bits]) && (I[pl_bits] <= R[pl_bits]) && (R[pl_bits] <= C[pl_bits]);
-  assume (0 <= I[data]) && (I[data] <= R[data]) && (R[data] <= C[data]);
-  assume (0 <= I[len]) && (I[len] <= R[len]) && (R[len] <= C[len]);
+  assume (0 <= I#[pl_bits]) && (I#[pl_bits] <= R#[pl_bits]) && (R#[pl_bits] <= C#[pl_bits]);
+  assume (0 <= I#[data]) && (I#[data] <= R#[data]) && (R#[data] <= C#[data]);
+  assume (0 <= I#[len]) && (I#[len] <= R#[len]) && (R#[len] <= C#[len]);
   assume AT#BvUle8(0bv8, octet_index);
   assume AT#BvUle8(octet_index, octet_count);
   assume octet_count == 14bv8;
@@ -289,7 +294,7 @@ procedure headerAdd#done#5()
   assert {:msg "headerAdd.cal(31.12): Action 'done' at headerAdd.cal(91.2) might not preserve the invariant (#35)"} (0 <= St) && (St <= 2);
 }
 procedure headerAdd##GuardWD#6()
-  modifies C, R, M, I, H, I#sub;
+  modifies C#, R#, M#, I#, H#, I#sub;
 {
   var pl_bits: Chan (bv8);
   var data: Chan (bv8);
@@ -308,14 +313,14 @@ procedure headerAdd##GuardWD#6()
   assume (St == 1) ==> AT#BvUle8(octet_index, 5bv8);
   assume (St == 2) ==> AT#BvUlt8(5bv8, octet_index);
   assume (0 <= St) && (St <= 2);
-  assert {:msg "headerAdd.cal(1.1): The actions 'send_header' and 'send_payload_octet' of actor 'headerAdd' might not have mutually exclusive guards (#36)"} !(true && true && AT#BvUlt8(octet_index, 5bv8) && (St == 1) && true && (1 <= (C[pl_bits] - R[pl_bits])) && AT#BvUlt8(octet_index, octet_count) && (St == 2));
-  assert {:msg "headerAdd.cal(1.1): The actions 'send_header' and 'get_data_len' of actor 'headerAdd' might not have mutually exclusive guards (#37)"} !(true && true && AT#BvUlt8(octet_index, 5bv8) && (St == 1) && true && (1 <= (C[pl_bits] - R[pl_bits])) && (St == 0));
-  assert {:msg "headerAdd.cal(1.1): The actions 'send_header' and 'done' of actor 'headerAdd' might not have mutually exclusive guards (#38)"} !(true && true && AT#BvUlt8(octet_index, 5bv8) && (St == 1) && true && (!((1 <= (C[pl_bits] - R[pl_bits])) && AT#BvUlt8(octet_index, octet_count) && (St == 2))) && true && (octet_index == octet_count) && (St == 2));
-  assert {:msg "headerAdd.cal(1.1): The actions 'send_header' and 'send_length' of actor 'headerAdd' might not have mutually exclusive guards (#39)"} !(true && true && AT#BvUlt8(octet_index, 5bv8) && (St == 1) && true && (!(true && AT#BvUlt8(octet_index, 5bv8) && (St == 1))) && true && (octet_index == 5bv8) && (St == 1));
-  assert {:msg "headerAdd.cal(1.1): The actions 'send_payload_octet' and 'get_data_len' of actor 'headerAdd' might not have mutually exclusive guards (#40)"} !(true && (1 <= (C[pl_bits] - R[pl_bits])) && AT#BvUlt8(octet_index, octet_count) && (St == 2) && true && (1 <= (C[pl_bits] - R[pl_bits])) && (St == 0));
-  assert {:msg "headerAdd.cal(1.1): The actions 'send_payload_octet' and 'done' of actor 'headerAdd' might not have mutually exclusive guards (#41)"} !(true && (1 <= (C[pl_bits] - R[pl_bits])) && AT#BvUlt8(octet_index, octet_count) && (St == 2) && true && (!((1 <= (C[pl_bits] - R[pl_bits])) && AT#BvUlt8(octet_index, octet_count) && (St == 2))) && true && (octet_index == octet_count) && (St == 2));
-  assert {:msg "headerAdd.cal(1.1): The actions 'send_payload_octet' and 'send_length' of actor 'headerAdd' might not have mutually exclusive guards (#42)"} !(true && (1 <= (C[pl_bits] - R[pl_bits])) && AT#BvUlt8(octet_index, octet_count) && (St == 2) && true && (!(true && AT#BvUlt8(octet_index, 5bv8) && (St == 1))) && true && (octet_index == 5bv8) && (St == 1));
-  assert {:msg "headerAdd.cal(1.1): The actions 'get_data_len' and 'done' of actor 'headerAdd' might not have mutually exclusive guards (#43)"} !(true && (1 <= (C[pl_bits] - R[pl_bits])) && (St == 0) && true && (!((1 <= (C[pl_bits] - R[pl_bits])) && AT#BvUlt8(octet_index, octet_count) && (St == 2))) && true && (octet_index == octet_count) && (St == 2));
-  assert {:msg "headerAdd.cal(1.1): The actions 'get_data_len' and 'send_length' of actor 'headerAdd' might not have mutually exclusive guards (#44)"} !(true && (1 <= (C[pl_bits] - R[pl_bits])) && (St == 0) && true && (!(true && AT#BvUlt8(octet_index, 5bv8) && (St == 1))) && true && (octet_index == 5bv8) && (St == 1));
-  assert {:msg "headerAdd.cal(1.1): The actions 'done' and 'send_length' of actor 'headerAdd' might not have mutually exclusive guards (#45)"} !(true && (!((1 <= (C[pl_bits] - R[pl_bits])) && AT#BvUlt8(octet_index, octet_count) && (St == 2))) && true && (octet_index == octet_count) && (St == 2) && true && (!(true && AT#BvUlt8(octet_index, 5bv8) && (St == 1))) && true && (octet_index == 5bv8) && (St == 1));
+  assert {:msg "headerAdd.cal(1.1): The actions 'get_data_len' and 'done' of actor 'headerAdd' might not have mutually exclusive guards (#36)"} !(true && (1 <= (C#[pl_bits] - R#[pl_bits])) && (St == 0) && true && (!((1 <= (C#[pl_bits] - R#[pl_bits])) && AT#BvUlt8(octet_index, octet_count) && (St == 2))) && true && (octet_index == octet_count) && (St == 2));
+  assert {:msg "headerAdd.cal(1.1): The actions 'get_data_len' and 'send_payload_octet' of actor 'headerAdd' might not have mutually exclusive guards (#37)"} !(true && (1 <= (C#[pl_bits] - R#[pl_bits])) && (St == 0) && true && (1 <= (C#[pl_bits] - R#[pl_bits])) && AT#BvUlt8(octet_index, octet_count) && (St == 2));
+  assert {:msg "headerAdd.cal(1.1): The actions 'get_data_len' and 'send_length' of actor 'headerAdd' might not have mutually exclusive guards (#38)"} !(true && (1 <= (C#[pl_bits] - R#[pl_bits])) && (St == 0) && true && (!(true && AT#BvUlt8(octet_index, 5bv8) && (St == 1))) && true && (octet_index == 5bv8) && (St == 1));
+  assert {:msg "headerAdd.cal(1.1): The actions 'get_data_len' and 'send_header' of actor 'headerAdd' might not have mutually exclusive guards (#39)"} !(true && (1 <= (C#[pl_bits] - R#[pl_bits])) && (St == 0) && true && true && AT#BvUlt8(octet_index, 5bv8) && (St == 1));
+  assert {:msg "headerAdd.cal(1.1): The actions 'done' and 'send_payload_octet' of actor 'headerAdd' might not have mutually exclusive guards (#40)"} !(true && (!((1 <= (C#[pl_bits] - R#[pl_bits])) && AT#BvUlt8(octet_index, octet_count) && (St == 2))) && true && (octet_index == octet_count) && (St == 2) && true && (1 <= (C#[pl_bits] - R#[pl_bits])) && AT#BvUlt8(octet_index, octet_count) && (St == 2));
+  assert {:msg "headerAdd.cal(1.1): The actions 'done' and 'send_length' of actor 'headerAdd' might not have mutually exclusive guards (#41)"} !(true && (!((1 <= (C#[pl_bits] - R#[pl_bits])) && AT#BvUlt8(octet_index, octet_count) && (St == 2))) && true && (octet_index == octet_count) && (St == 2) && true && (!(true && AT#BvUlt8(octet_index, 5bv8) && (St == 1))) && true && (octet_index == 5bv8) && (St == 1));
+  assert {:msg "headerAdd.cal(1.1): The actions 'done' and 'send_header' of actor 'headerAdd' might not have mutually exclusive guards (#42)"} !(true && (!((1 <= (C#[pl_bits] - R#[pl_bits])) && AT#BvUlt8(octet_index, octet_count) && (St == 2))) && true && (octet_index == octet_count) && (St == 2) && true && true && AT#BvUlt8(octet_index, 5bv8) && (St == 1));
+  assert {:msg "headerAdd.cal(1.1): The actions 'send_payload_octet' and 'send_length' of actor 'headerAdd' might not have mutually exclusive guards (#43)"} !(true && (1 <= (C#[pl_bits] - R#[pl_bits])) && AT#BvUlt8(octet_index, octet_count) && (St == 2) && true && (!(true && AT#BvUlt8(octet_index, 5bv8) && (St == 1))) && true && (octet_index == 5bv8) && (St == 1));
+  assert {:msg "headerAdd.cal(1.1): The actions 'send_payload_octet' and 'send_header' of actor 'headerAdd' might not have mutually exclusive guards (#44)"} !(true && (1 <= (C#[pl_bits] - R#[pl_bits])) && AT#BvUlt8(octet_index, octet_count) && (St == 2) && true && true && AT#BvUlt8(octet_index, 5bv8) && (St == 1));
+  assert {:msg "headerAdd.cal(1.1): The actions 'send_length' and 'send_header' of actor 'headerAdd' might not have mutually exclusive guards (#45)"} !(true && (!(true && AT#BvUlt8(octet_index, 5bv8) && (St == 1))) && true && (octet_index == 5bv8) && (St == 1) && true && true && AT#BvUlt8(octet_index, 5bv8) && (St == 1));
 }
